. (#1)

LeanYjs.lean
@@ -2,42 +2,83 @@
 -- Import modules here that should be built as part of the library.
 import LeanYjs.Basic
 
+variable (A : Type) [BEq A]
+
 def ActorId := Nat
 
 instance : LT ActorId where
   lt x y := Nat.lt x y
 
-instance ActorIdOfNat n: OfNat ActorId n where
+instance : DecidableRel (· < · : ActorId → ActorId → Prop) := by
+  intros x y
+  unfold ActorId at x y
+  apply (inferInstance : Decidable (x < y))
+
+instance ActorIdOfNat n : OfNat ActorId n where
   ofNat := n
 
-inductive YjsItem (A : Type): Type where
-| item: (origin: YjsItem A) -> (rightOrigin: YjsItem A) -> ActorId -> A -> YjsItem A
-| first: YjsItem A
-| last: YjsItem A
+mutual
+inductive YjsPtr : Type where
+| itemPtr : YjsItem -> YjsPtr
+| first : YjsPtr
+| last : YjsPtr
 
-def YjsItem.origin {A : Type}: YjsItem A -> Option (YjsItem A)
+inductive YjsItem : Type where
+| item : (origin : YjsPtr) -> (rightOrigin : YjsPtr) -> ActorId -> A -> YjsItem
+end
+
+instance : BEq ActorId where
+  beq x y := by
+    unfold ActorId at x y
+    apply Nat.beq x y
+
+mutual
+def yjsItemEq (x y : YjsItem A) : Bool :=
+  match x, y with
+  | YjsItem.item origin1 rightOrigin1 id1 c1, YjsItem.item origin2 rightOrigin2 id2 c2 =>
+    yjsPtrEq origin1 origin2 && yjsPtrEq rightOrigin1 rightOrigin2 && id1 == id2 && c1 == c2
+
+def yjsPtrEq (x y : YjsPtr A) : Bool :=
+  match x, y with
+  | YjsPtr.itemPtr item1, YjsPtr.itemPtr item2 => yjsItemEq item1 item2
+  | YjsPtr.first, YjsPtr.first => true
+  | YjsPtr.last, YjsPtr.last => true
+  | _, _ => false
+end
+
+instance BEqYjsItem : BEq (YjsItem A) where
+  beq := yjsItemEq _
+
+instance BEqYjsPtr : BEq (@YjsPtr A) where
+  beq := yjsPtrEq _
+
+instance : Coe (YjsItem A) (YjsPtr A) where
+  coe item := YjsPtr.itemPtr item
+
+def YjsItem.origin {A : Type} : YjsItem A -> YjsPtr A
 | YjsItem.item origin _  _ _ => origin
-| _ => none
 
-def YjsItem.rightOrigin {A : Type}: YjsItem A -> Option (YjsItem A)
+def YjsItem.rightOrigin {A : Type} : YjsItem A -> YjsPtr A
 | YjsItem.item _ rightOrigin _ _ => rightOrigin
-| _ => none
 
-inductive YjsLessThan1 (A : Type): YjsItem A -> YjsItem A -> Prop where
-| ltFirst: forall (left right: YjsItem A) (c: A), YjsLessThan1 A YjsItem.first (YjsItem.item left right _ c)
-| ltLast: forall (left right: YjsItem A) (c: A), YjsLessThan1 A (YjsItem.item left right _ c) YjsItem.last
-| ltOrigin: forall (item right: YjsItem A) (id: ActorId) (c: A), YjsLessThan1 A item (YjsItem.item item right id c)
-| ltRightOrigin: forall (item left: YjsItem A) (id: ActorId) (c: A), YjsLessThan1 A (YjsItem.item left item id c) item
+def YjsItem.id {A : Type} : YjsItem A -> ActorId
+| YjsItem.item _ _ id _ => id
+
+inductive YjsLessThan1 (A : Type) : YjsItem A -> YjsItem A -> Prop where
+| ltOrigin : forall (item : YjsItem A) (right : YjsPtr A) (id : ActorId) (c : A),
+    YjsLessThan1 A item (YjsItem.item (YjsPtr.itemPtr item) right id c)
+| ltRightOrigin : forall (item : YjsItem A) (left : YjsPtr A) (id : ActorId) (c : A),
+    YjsLessThan1 A (YjsItem.item left (YjsPtr.itemPtr item) id c) item
 
 /- transitive closure -/
-inductive YjsLessThanTr {a : Type}: YjsItem a -> YjsItem a -> Prop where
-| base: forall (item1 item2: YjsItem a), YjsLessThan1 a item1 item2 -> YjsLessThanTr item1 item2
-| trans: forall (item1 item2 item3: YjsItem a), YjsLessThanTr item1 item2 -> YjsLessThan1 a item2 item3 -> YjsLessThanTr item1 item3
+inductive YjsLessThanTr {a : Type} : YjsItem a -> YjsItem a -> Prop where
+| base : forall (item1 item2 : YjsItem a), YjsLessThan1 a item1 item2 -> YjsLessThanTr item1 item2
+| trans : forall (item1 item2 item3 : YjsItem a), YjsLessThanTr item1 item2 -> YjsLessThan1 a item2 item3 -> YjsLessThanTr item1 item3
 
-inductive YjsLessThan {a : Type}: YjsItem a -> YjsItem a -> Prop where
-| ltOrigin: forall item1 item2, YjsLessThanTr item1 item2 -> YjsLessThan item1 item2
-| ltTr: forall item1 item2 item3, YjsLessThan item1 item2 -> YjsLessThan item2 item3 -> YjsLessThan item1 item3
-| lt1: forall (left1 left2 right1 right2: YjsItem a) (id1 id2: ActorId) (c1 c2: a),
+inductive YjsLessThan {A : Type} : YjsItem A -> YjsItem A -> Prop where
+| ltOrigin : forall item1 item2, YjsLessThanTr item1 item2 -> YjsLessThan item1 item2
+| ltTr : forall item1 item2 item3, YjsLessThan item1 item2 -> YjsLessThan item2 item3 -> YjsLessThan item1 item3
+| lt1 : forall (left1 left2 right1 right2 : YjsItem A) (id1 id2 : ActorId) (c1 c2 : A),
     item1 = YjsItem.item left1 right1 id1 c1
     -> item2 = YjsItem.item left2 right2 id2 c2
     /- left1 < item2 < right1 -/
@@ -47,7 +88,7 @@ inductive YjsLessThan {a : Type}: YjsItem a -> YjsItem a -> Prop where
     /- left2 < item1 -/
     -> YjsLessThan left2 item1
     -> YjsLessThan item2 item1
-| lt2: forall (left1 left2 right1 right2: YjsItem a) (id1 id2: ActorId) (c1 c2: a),
+| lt2 : forall (left1 left2 right1 right2 : YjsItem A) (id1 id2 : ActorId) (c1 c2 : A),
     item1 = YjsItem.item left1 right1 id1 c1
     -> item2 = YjsItem.item left2 right2 id2 c2
     /- left1 < item2 < right1 -/
@@ -55,42 +96,41 @@ inductive YjsLessThan {a : Type}: YjsItem a -> YjsItem a -> Prop where
     /- left2 < left1 -/
     -> YjsLessThanTr left2 left1
     -> YjsLessThan item1 item2
-| ltSame1: forall (left right: YjsItem a) (id1 id2: ActorId) (c1 c2: a),
+| ltId1 : forall (left right1 right2 : YjsItem A) (id1 id2 : ActorId) (c1 c2 : A),
+    item1 = YjsItem.item left right1 id1 c1
+    -> item2 = YjsItem.item left right2 id2 c2
+    -> YjsLessThan item1 right2
+    -> id1 < id2
+    -> YjsLessThan item1 item2
+| ltId2 : forall (left right : YjsPtr A) (id1 id2 : ActorId) (c1 c2 : A),
     item1 = YjsItem.item left right id1 c1
     -> item2 = YjsItem.item left right id2 c2
     -> id1 < id2
     -> YjsLessThan item1 item2
-| ltSame2: forall (left right: YjsItem a) (id1 id2: ActorId) (c1 c2: a),
-    item1 = YjsItem.item left right id1 c1
-    -> item2 = YjsItem.item left right id2 c2
-    -> id2 < id1
-    -> YjsLessThan item2 item1
-  -- same origin, different right origin
-| ltSame3: forall (left right1 right2: YjsItem a) (id1 id2: ActorId) (c1 c2: a),
+| ltId3 : forall (left : YjsPtr A) (right1 right2 : YjsItem A) (id1 id2 : ActorId) (c1 c2 : A),
     item1 = YjsItem.item left right1 id1 c1
     -> item2 = YjsItem.item left right2 id2 c2
     -> id1 < id2
     /- left < item2 < right1 -/
     -> YjsLessThan item2 right1
     -> YjsLessThan item1 right2
-
     -> YjsLessThan item1 item2
 
 namespace ex1
   open Nat
-  def item1 := YjsItem.item YjsItem.first YjsItem.last 1 1
-  def item2 := YjsItem.item YjsItem.first YjsItem.last 2 2
+  def item1 := YjsItem.item YjsPtr.first YjsPtr.last 1 1
+  def item2 := YjsItem.item YjsPtr.first YjsPtr.last 2 2
 
   example : YjsLessThan item1 item2 :=
   by
-    apply @YjsLessThan.ltSame1 (item1 := item1) (item2 := item2) <;> try rfl
+    apply @YjsLessThan.ltId2 (item1 := item1) (item2 := item2) <;> try rfl
     simp [ActorId]
 end ex1
 
 namespace ex2
-  def item0 := YjsItem.item YjsItem.first YjsItem.last 0 0
-  def item1 := YjsItem.item YjsItem.first YjsItem.last 1 1
-  def item2 := YjsItem.item YjsItem.first item0 2 2
+  def item0 := YjsItem.item YjsPtr.first YjsPtr.last 0 0
+  def item1 := YjsItem.item YjsPtr.first YjsPtr.last 1 1
+  def item2 := YjsItem.item YjsPtr.first item0 2 2
 
   example : YjsLessThan item2 item1 :=
   by
@@ -98,20 +138,61 @@ namespace ex2
     . apply YjsLessThan.ltOrigin
       apply YjsLessThanTr.base
       apply YjsLessThan1.ltRightOrigin
-    . apply YjsLessThan.ltSame1 <;> try rfl
+    . apply YjsLessThan.ltId2 <;> try rfl
       unfold ActorId
       decide
 end ex2
-  example : Not (YjsLessThan item1 item2) :=
-  by
-    intro h
-    cases h
-    . case ltOrigin t =>
-      cases t
-      .
-    case ltTr => done
-    case lt1 => done
-    case lt2 => done
-    case ltSame1 => done
-    case ltSame2 => done
-    case ltSame3 => done
+
+inductive IntegrateError where
+| notFound : IntegrateError
+
+variable {A: Type} [BEq A]
+
+def findIdx (p : YjsPtr A) (arr : Array (YjsItem A)) : Except IntegrateError Int :=
+  match p with
+  | YjsPtr.itemPtr item =>
+    match Array.findIdx? (fun i => i == item) arr with
+    | some idx => return idx
+    | none => Except.error IntegrateError.notFound
+  | YjsPtr.first => return 0
+  | YjsPtr.last => return (Array.size arr - 1)
+
+def getExcept (arr : Array (YjsItem A)) (idx : Nat) : Except IntegrateError (YjsItem A) :=
+  match Array.get? arr idx with
+  | some item => return item
+  | none => Except.error IntegrateError.notFound
+
+inductive LoopCommand (A : Type) where
+| Continue : A -> LoopCommand A
+| Break : A -> LoopCommand A
+
+def fold_range {M : Type -> Type} [Monad M] {A : Type} (a b : Nat) (f : A → Nat → M (LoopCommand (M A))) (acc : M A) : M A := do
+  if a ≥ b then acc
+  else
+    let acc <- acc
+    let cmd <- f acc a
+    match cmd with
+    | LoopCommand.Continue acc => fold_range (a + 1) b f acc
+    | LoopCommand.Break acc => acc
+  termination_by (b - a)
+
+def integrate (newItem : YjsItem A) (arr : Array (YjsItem A)) : Except IntegrateError (Array (YjsItem A)) := do
+  let leftIdx <- findIdx (YjsItem.origin newItem) arr
+  let rightIdx <- findIdx (YjsItem.rightOrigin newItem) arr
+  let (_, i) <- fold_range (Int.toNat (leftIdx + 1)) (Int.toNat rightIdx) (acc := Except.ok (false, leftIdx + 1)) (fun acc i => do
+    let (scanning, leftIdx) := acc
+    let oItem <- getExcept arr i
+    let oLeftIdx <- findIdx oItem.origin arr
+    let oRightIdx <- findIdx oItem.rightOrigin arr
+    if oLeftIdx < leftIdx then
+      return LoopCommand.Break (return (true, i))
+    else if oLeftIdx == leftIdx then
+      if decide (YjsItem.id newItem > YjsItem.id oItem) then
+        return (LoopCommand.Continue (return (false, i + 1)))
+      else if oRightIdx == rightIdx then
+        return (LoopCommand.Break (return (false, i + 1)))
+      else
+        return (LoopCommand.Continue (return (true, i + 1)))
+    else
+      return ((LoopCommand.Continue (return (scanning, i + 1)))))
+  return (Array.insertIdxIfInBounds arr (Int.toNat i) newItem)
